+\section{Formal Semantics}
\subsection{Transition System}

\begin{center}
$at = \text{ActorTypes} \rightharpoonup \text{Stm}$

$aEnv = \text{Anames} \rightharpoonup sEnv$

$sEnv = \text{Symbols} \rightharpoonup \text{Stm} \times \text{Symbols}$

$st = \text{Structs} \rightharpoonup \text{Symbols}$
\end{center}

\subsection{Expressions}
\subsubsection{Arithmetic}
\begin{align*}
&\inference[$\text{ADD}_\text{L}$]{sEnv \vdash a_1 \Rightarrow_A a_1'}
                    {sEnv \vdash  a_1 + a_2 \Rightarrow_A a_1' + a_2}
&
&\inference[$\text{ADD}_\text{R}$]{sEnv\vdash a_1 \Rightarrow_A a_1'}
                    {sEnv\vdash a_2 + a_1 \Rightarrow_A a_2 + a_1'}
\\\\
&\inference[$\text{ADD}_\text{V}$]{}
                    {v_1 + v_2 \Rightarrow_A v}
                    {, v_1 + v_2 = v}
\\\\
&\inference[$\text{SUB}_\text{L}$]{sEnv\vdash a_1 \Rightarrow_A a_1'}
                    {sEnv\vdash a_1 - a_2 \Rightarrow_A a_1' - a_2}
&
&\inference[$\text{SUB}_\text{R}$]{sEnv\vdash a_1 \Rightarrow_A a_1'}
                    {sEnv\vdash a_2 - a_1 \Rightarrow_A a_2 - a_1'}
\\\\
&\inference[$\text{SUB}_\text{V}$]{}
                    {v_1 - v_2 \Rightarrow_A v}
                    {, v_1 - v_2 = v}
\\\\
&\inference[$\text{MULT}_\text{L}$]{sEnv\vdash a_1 \Rightarrow_A a_1'}
                     {sEnv\vdash a_1 * a_2 \Rightarrow_A a_1' * a_2}
&
&\inference[$\text{MULT}_\text{R}$]{sEnv\vdash a_1 \Rightarrow_A a_1'}
                     {sEnv\vdash a_2 * a_1 \Rightarrow_A a_2 * a_1'}
\\\\
&\inference[$\text{MULT}_\text{V}$]{}
                     {v_1 * v_2 \Rightarrow_A v}
                     {, v_1 * v_2 = v}
\\\\
&\inference[$\text{DIV}_\text{L}$]{sEnv\vdash a_1 \Rightarrow_A a_1'}
                    {sEnv\vdash a_1 / a_2 \Rightarrow_A a_1' / a_2}
&
&\inference[$\text{DIV}_\text{R}$]{sEnv\vdash a_1 \Rightarrow_A a_1'}
                    {sEnv\vdash a_2 / a_1 \Rightarrow_A a_2 / a_1'}
\\\\
&\inference[$\text{DIV}_\text{V}$]{}
                    {v_1 / v_2 \Rightarrow_A v}
                    {, \frac{v_1}{v_2} = v}
\\\\
&\inference[$\text{MOD}_\text{L}$]{sEnv\vdash a_1 \Rightarrow_A a_1'}
                    {sEnv\vdash a_1 \% a_2 \Rightarrow_A a_1' \% a_2}
&
&\inference[$\text{MOD}_\text{R}$]{sEnv\vdash a_1 \Rightarrow_A a_1'}
                    {sEnv\vdash a_2 \% a_1 \Rightarrow_A a_2 \% a_1'}
\\\\
&\inference[$\text{MOD}_\text{V}$]{}
                    {v_1 \% v_2 \Rightarrow_A v}
                    {, v_1 \;\; \textrm{mod} \;\; v_2 = v}
\\\\
&\inference[$\text{POW}_\text{L}$]{sEnv\vdash a_1  \Rightarrow_A a_1'}
                    {sEnv\vdash a_1 \Twedge a_2 \Rightarrow_A a_1' \Twedge a_2}
&
&\inference[$\text{POW}_\text{R}$]{sEnv\vdash a_1 \Rightarrow_A a_1'}
                    {sEnv\vdash a_2 \Twedge a_1 \Rightarrow_A a_2 \Twedge a_1'}
\\\\
&\inference[$\text{POW}_\text{V}$]{}
                    {v_1 \Twedge v_2 \Rightarrow_A v}
                    {, v_1 ^ {v_2} = v}
\\\\
&\inference[$\text{ROOT}_\text{L}$]{sEnv\vdash a_1 \Rightarrow_A a_1'}
                    {sEnv\vdash a_1 \# a_2 \Rightarrow_A a_1' \# a_2}
&
&\inference[$\text{ROOT}_\text{R}$]{sEnv\vdash a_1 \Rightarrow_A a_1'}
                    {sEnv\vdash a_2 \# a_1 \Rightarrow_A a_2 \# a_1'}
\\\\
&\inference[$\text{ROOT}_\text{V}$]{}
                    {v_1 \# v_2 \Rightarrow_A v}
                    {, \sqrt[v_1]{v_2} = v}
\\\\
&\inference[$\text{PARENS}_\text{A}$]{sEnv\vdash a_1 \Rightarrow_A a_1'}
                       {sEnv\vdash (a_1) \Rightarrow_A (a_1')}
&
&\inference[$\text{PARENS}_\text{V}$]{}
                       {(v) \Rightarrow_A v}
\end{align*}
\subsubsection{Boolean}
\begin{align*}
&\inference[$\text{AND}_1$]{e \vdash b_1 \Rightarrow_B \bot}
                           {e \vdash b_1 \Tand b_2 \Rightarrow_B \bot}
\\\\
&\inference[$\text{AND}_2$]{e \vdash b_1 \Rightarrow_B \top \\ b_2 \Rightarrow_B \bot}
                           {e \vdash b_1 \Tand b_2 \Rightarrow_B \bot}
\\\\
&\inference[$\text{AND}_3$]{e \vdash b_1 \Rightarrow_B \top \\ b_2 \Rightarrow_B \top}
                           {e \vdash b_1 \Tand b_2 \Rightarrow_B \top}
\\\\
&\inference[OR]{}
               {e \vdash b_1 \Tor b_2 \Rightarrow_B \Tnot(\Tnot b_1 \Tand \Tnot b_2)}
\\\\
&\inference[XOR]{}
                  {e \vdash b_1 \Txor b_2 \Rightarrow_B (\Tnot(b_1 \Tand b_2)) \Tand (b_1 \Tor b_2)}
\\\\
&\inference[NOR]{}
                {e \vdash b_1 \Tnor b_2 \Rightarrow_B \Tnot( b_1 \Tor b_2 )}
\\\\
&\inference[$\text{NOT}_\top$]{e \vdash b_1 \Rightarrow_B \top}
                              {e \vdash \Tnot b_1 \Rightarrow_B \bot}
\\\\
&\inference[$\text{NOT}_\bot$]{e \vdash b_1 \Rightarrow_B \bot}
                              {e \vdash \Tnot b_1 \Rightarrow_B \top}
\\\\
&\inference[NAND]{}
                   {e \vdash b_1 \Tnand b_2 \Rightarrow_B \Tnot( b_1 \Tand b_2 )}
\\\\
&\inference[TRUE]{}
                   {\Braket{\Ttrue,sEnv} \Rightarrow_B \top}
&\inference[FALSE]{}
                   {\Braket{\Tfalse,sEnv} \Rightarrow_B \bot}
\end{align*}
\subsubsection{Logical}
\begin{align*}
&\inference[$\text{EQUALS}_\text{L}$]{e \vdash a_1 \Rightarrow_B a_1'}
                    {e \vdash a_1 = a_2 \Rightarrow_B a_1' = a_2}
&
&\inference[$\text{EQUALS}_\text{R}$]{e \vdash a_1 \Rightarrow_B a_1'}
                    {e \vdash a_2 = a_1 \Rightarrow_B a_2 = a_1'}
\\\\
&\inference[$\text{EQUALS}_\text{V1}$]{}
                    {v_1 = v_2 \Rightarrow_B \top}
                    {, v_1 = v_2}
&
&\inference[$\text{EQUALS}_\text{V2}$]{}
                    {v_1 = v_2 \Rightarrow_B \bot}
                    {, v_1 \neq v_2}
\\\\
&\inference[$\text{EQUALS}_\text{Actor}$]{a(act_1) = e\\ a(act_2) = e}
                    {act_1 = act_2 \Rightarrow_B \top}
&
&\inference[$\text{EQUALS}_\text{Actor}$]{a(act_1) = e\\ a(act_2) = e'}
                    {act_1 = act_2 \Rightarrow_B \bot}
                    {e \neq e'}
\\\\
&\inference[$NEQUALS$]{}
                    {e \vdash a_1 != a_2 \Rightarrow_B \Tnot (a_1 = a_2)}
&\inference[$\text{LT}_\text{L}$]{e \vdash a_1 \Rightarrow_A a_1'}
                    {e \vdash a_1 < a_2 \Rightarrow_A a_1' < a_2}
&
&\inference[$\text{LT}_\text{R}$]{e \vdash a_1 \Rightarrow_A a_1'}
                    {e \vdash a_2 < a_1 \Rightarrow_A a_2 < a_1'}
\\\\
&\inference[$\text{LT}_\text{V1}$]{}
                    {v_1 < v_2 \Rightarrow_B \top}
                    {, v_1 < v_2}
&
&\inference[$\text{LT}_\text{V2}$]{}
                    {v_1 < v_2 \Rightarrow_B \bot}
                    {, v_1 \geq v_2}
\end{align*}
\subsection{Statements}

\subsection{Actors}
